add counting arguments to invariant

examples/scache/RWLock.i.dfy
@@ -3,6 +3,7 @@ include "../../lib/Lang/NativeTypes.s.dfy"
 include "Constants.i.dfy"
 include "ResourceBuilderSpec.s.dfy"
 include "CacheResources.i.dfy"
+include "Multisets.i.dfy"
 
 module RWLock refines ResourceBuilderSpec {
   import Ptrs
@@ -10,10 +11,12 @@ module RWLock refines ResourceBuilderSpec {
   import opened NativeTypes
   import opened Constants
   import opened Options
+  import opened MultisetUtil
 
   datatype Key = Key(data_ptr: Ptrs.Ptr, idx_ptr: Ptrs.Ptr, cache_idx: int)
 
   linear datatype Handle = CacheEntryHandle(
+      key: Key,
       linear cache_entry: CacheResources.R,
       linear data: Ptrs.ArrayDeref<byte>,
       linear idx: Ptrs.Deref<int>
@@ -21,6 +24,7 @@ module RWLock refines ResourceBuilderSpec {
   {
     predicate is_handle(key: Key)
     {
+      && this.key == key
       && this.cache_entry.CacheEntry?
       && this.cache_entry.cache_idx == key.cache_idx
       && this.data.ptr == key.data_ptr
@@ -59,7 +63,7 @@ module RWLock refines ResourceBuilderSpec {
 
   datatype ExcState = 
     | WLSNone
-    | WLSPendingAwaitWriteBack
+    | WLSPendingAwaitWriteBack(t: int)
     | WLSPending(t: int, visited: int, clean: bool)
     | WLSObtained(t: int, clean: bool)
 
@@ -117,15 +121,16 @@ module RWLock refines ResourceBuilderSpec {
   datatype BasicStep =
     | TakeWriteBackStep(flags: R, flags': R, r': R, handle': R)
     | ReleaseWriteBackStep(flags: R, r: R, handle: R, flags': R, fl: Flag)
+    | TakeExcLockFinishWriteBackStep(flags: R, r: R, flags': R, r': R,
+          t: int, fl: Flag, clean: bool)
+    | TakeExcLockSharedLockZeroStep(rc_rc': R, r: R, r': R,
+          t: int, idx: int, clean: bool)
+    | TakeExcLockFinishStep(r: R, r': R, handle': R, t: int, clean: bool) 
 
   predicate TakeWriteBack(
-    key: Key,
-    state: RWLockState,
-    state': RWLockState,
+    key: Key, state: RWLockState, state': RWLockState,
     flags: R,
-    flags': R,
-    r': R,
-    handle': R)
+    flags': R, r': R, handle': R)
   {
     && state' == state.(backHeld := true)
     && flags == Internal(FlagsField(key, Available))
@@ -136,12 +141,8 @@ module RWLock refines ResourceBuilderSpec {
   }
 
   predicate ReleaseWriteBack(
-    key: Key,
-    state: RWLockState,
-    state': RWLockState,
-    flags: R,
-    r: R,
-    handle: R,
+    key: Key, state: RWLockState, state': RWLockState,
+    flags: R, r: R, handle: R,
     flags': R,
     fl: Flag)
   {
@@ -153,6 +154,48 @@ module RWLock refines ResourceBuilderSpec {
     && (fl == WriteBack_PendingExcLock ==>
         flags' == Internal(FlagsField(key, PendingExcLock)))
     && handle.Const? && handle.v.is_handle(key)
+  }
+
+  predicate TakeExcLockFinishWriteBack(
+    key: Key, state: RWLockState, state': RWLockState,
+    flags: R, r: R,
+    flags': R, r': R,
+    t: int, fl: Flag, clean: bool)
+  {
+    && fl != WriteBack && fl != WriteBack_PendingExcLock
+    && state' == state.(excState := WLSPending(t, 0, clean))
+    && flags == Internal(FlagsField(key, fl))
+    && r == Internal(ExcLockPendingAwaitWriteBack(key, t))
+    && flags' == Internal(FlagsField(key,
+          if clean then ExcLock_Clean else ExcLock_Dirty))
+    && r' == Internal(ExcLockPending(key, t, 0, clean))
+  }
+
+  predicate TakeExcLockSharedLockZero(
+    key: Key, state: RWLockState, state': RWLockState,
+    rc_rc': R,
+    r: R, r': R,
+    t: int, idx: int, clean: bool)
+  {
+    && state' == state.(excState := WLSPending(t, idx + 1, clean))
+    && rc_rc' == Internal(SharedLockRefCount(key, idx,
+        if t == idx then 1 else 0))
+    && r == Internal(ExcLockPending(key, t, idx, clean))
+    && r' == Internal(ExcLockPending(key, t, idx + 1, clean))
+  }
+
+  predicate TakeExcLockFinish(
+    key: Key, state: RWLockState, state': RWLockState,
+    r: R,
+    r': R, handle': R,
+    t: int, clean: bool)
+  {
+    && state' == state
+        .(excState := WLSObtained(t, clean))
+        .(handle := None)
+    && r == Internal(ExcLockPending(key, t, NUM_THREADS, clean))
+    && r' == Internal(ExcLockObtained(key, t, clean))
+    && (state.handle.Some? ==> handle' == Exc(state.handle.value))
   }
 
   datatype QStep =
@@ -180,130 +223,39 @@ module RWLock refines ResourceBuilderSpec {
         && step.a' == multiset{flags'}
         && ReleaseWriteBack(step.key, step.state, step.state',
             flags, r, handle, flags', fl)
+      case TakeExcLockFinishWriteBackStep(flags, r, flags', r', t, fl, clean) =>
+        && step.a == multiset{flags, r}
+        && step.a' == multiset{flags', r'}
+        && TakeExcLockFinishWriteBack(step.key, step.state, step.state',
+            flags, r, flags', r', t, fl, clean)
+      case TakeExcLockSharedLockZeroStep(rc_rc', r, r', t, idx, clean) =>
+        && step.a == multiset{r, rc_rc'}
+        && step.a' == multiset{r', rc_rc'}
+        && TakeExcLockSharedLockZero(step.key, step.state, step.state', rc_rc', r, r', t, idx, clean)
+      case TakeExcLockFinishStep(r, r', handle', t, clean) =>
+        && step.a == multiset{r}
+        && step.a' == multiset{r',handle'}
+        && TakeExcLockFinish(step.key, step.state, step.state', r, r', handle', t, clean)
     }
   }
 
-  /*predicate TakeWriteBack(a: multiset<R>, b: multiset<R>, key: Key,
-      g: map<Key, RWLockState>, g': map<Key, RWLockState>)
-  {
-    && key in g
-    && key in g'
-    && g' == g[key := g'[key]]
-    && g'[key] == g[key].(backHeld := true)
-    && a == multiset{
-      Internal(Global(g)),
-      Internal(FlagsField(key, Available))
-    }
-    && b == multiset{
-      Internal(Global(g')),
-      Internal(FlagsField(key, WriteBack)),
-      Internal(WriteBackObtained(key))
-    }
-  }*/
-
-  /*predicate TakeExcLock(a: multiset<Q>, b: multiset<Q>, key: Key)
-  {
-    && a == multiset{ FlagsField(key, Available) }
-    && b == multiset{
-      FlagsField(key, ExcLock),
-      ExcLockPendingAwaitWriteBack(key)
-    }
-  }
-
-  predicate TakeExcLockAwaitWriteBack(a: multiset<Q>, b: multiset<Q>, key: Key)
-  {
-    && a == multiset{ FlagsField(key, WriteBack) }
-    && b == multiset{
-      FlagsField(key, WriteBack_PendingExcLock),
-      ExcLockPendingAwaitWriteBack(key)
-    }
-  }
-
-  predicate TakeExcLockFinishWriteBack(a: multiset<Q>, b: multiset<Q>, key: Key, fl: Flag)
-  {
-    // The 'free' case cannot actually occur, but it's convenient to allow it.
-    && (fl == ExcLock || fl == Available)
-    && a == multiset{
-      FlagsField(key, fl),
-      ExcLockPendingAwaitWriteBack(key)
-    }
-    && b == multiset{
-      FlagsField(key, fl),
-      ExcLockPending(key, 0)
-    }
-  }
-
-  predicate TakeExcLockCheckSharedLockZero(a: multiset<Q>, b: multiset<Q>, key: Key, idx: int)
-  {
-    && a == multiset{
-      ExcLockPending(key, idx),
-      SharedLockRefCount(key, idx, 0) 
-    }
-    && b == multiset{
-      ExcLockPending(key, idx + 1),
-      SharedLockRefCount(key, idx, 0) 
-    }
-  }
-
-  predicate TakeExcLockFinish(a: multiset<Q>, b: multiset<Q>, key: Key)
-  {
-    && a == multiset{
-      ExcLockPending(key, NUM_THREADS)
-    }
-    && b == multiset{
-      ExcLockObtained(key)
-    }
-  }*/
-
-  /*
-  predicate TakeSharedLock(a: multiset<Q>, b: multiset<Q>, key: Key, t: int, r: uint8)
-  {
-    && a == multiset{
-      SharedLockRefCount(key, t, r)
-    }
-    && a == multiset{
-      SharedLockRefCount(key, t, if r == 255 then 0 else r+1),
-      SharedLockPending(key, t)
-    }
-  }
-
-  predicate TakeSharedLockFinish(a: multiset<Q>, b: multiset<Q>, key: Key, t: int, r: uint8, fl: Flag)
-  {
-    && (fl == Available || fl == WriteBack)
-    && a == multiset{
-      SharedLockPending(key, t),
-      FlagsField(key, fl)
-    }
-    && a == multiset{
-      SharedLockObtained(key, t)
-    }
-  }
-
-  predicate TakeSharedLockBail(a: multiset<Q>, b: multiset<Q>, key: Key, t: int, r: uint8)
-  {
-    && a == multiset{
-      SharedLockRefCount(key, t, r),
-      SharedLockPending(key, t)
-    }
-    && b == multiset{
-      SharedLockRefCount(key, t, if r == 0 then 255 else r-1)
-    }
-  }*/
-
-  predicate InvRWLockState(key: Key, state: RWLockState)
+  predicate InvRWLockState(key: Key, state: RWLockState, m: multiset<R>)
   {
     && |state.readCounts| == NUM_THREADS
     && (state.excState.WLSPendingAwaitWriteBack? ==>
         && state.readState == RSNone
         && !state.unmapped
+        && 0 <= state.excState.t < NUM_THREADS
       )
     && (state.excState.WLSPending? ==>
       && state.readState == RSNone
       && !state.unmapped
       && !state.backHeld
-      && 0 <= state.excState.visited < NUM_THREADS
+      && 0 <= state.excState.visited <= NUM_THREADS
       && (forall i | 0 <= i < state.excState.visited
-          :: state.readCounts[i] == 0)
+          && i != state.excState.t :: state.readCounts[i] == 0)
+      && (0 <= state.excState.t < state.excState.visited ==>
+            state.readCounts[state.excState.t] == 1)
       && 0 <= state.excState.t < NUM_THREADS
     )
     && (state.excState.WLSObtained? ==>
@@ -311,7 +263,9 @@ module RWLock refines ResourceBuilderSpec {
       && !state.unmapped
       && !state.backHeld
       && (forall i | 0 <= i < |state.readCounts|
-          :: state.readCounts[i] == 0)
+          && i != state.excState.t :: state.readCounts[i] == 0)
+      && (0 <= state.excState.t < |state.readCounts| ==>
+            state.readCounts[state.excState.t] == 1)
       && 0 <= state.excState.t < NUM_THREADS
     )
     && (state.backHeld ==>
@@ -341,16 +295,63 @@ module RWLock refines ResourceBuilderSpec {
     )
     && (state.excState.WLSObtained? ==> state.handle.None?)
     && (!state.excState.WLSObtained? ==> state.handle.Some?)
+    && (state.handle.Some? ==>
+      state.handle.value.is_handle(key)
+    )
+    && (forall i | 0 <= i < |state.readCounts|
+      :: state.readCounts[i] == CountCountedRefs(m, key, i))
   }
 
-  predicate InvGlobal(g: map<Key, RWLockState>)
+  predicate is_counted_ref(r: R, key: Key, t: int)
   {
-    forall key | key in g :: InvRWLockState(key, g[key])
+    && r.Internal?
+    && (r.q.SharedLockPending? || r.q.SharedLockPending2?
+        || r.q.SharedLockObtained?
+        || r.q.ExcLockPendingAwaitWriteBack?
+        || r.q.ExcLockPending?
+        || r.q.ExcLockObtained?
+        || r.q.ReadingPendingCounted?
+        || r.q.ReadingObtained?)
+    && r.q.key == key
+    && r.q.t == t
+  }
+
+  function CountCountedRefs(m: multiset<R>, key: Key, i: int) : nat
+  {
+    MultisetUtil.Count((r) => is_counted_ref(r, key, i), m)
+  }
+
+  predicate is_const_ref(r: R, key: Key)
+  {
+    && r.Internal?
+    && (r.q.SharedLockObtained? || r.q.WriteBackObtained?)
+    && r.q.key == key
+  }
+
+  function CountConstRefs(m: multiset<R>, key: Key) : nat
+  {
+    MultisetUtil.Count((r) => is_const_ref(r, key), m)
+  }
+
+  predicate is_const(r: R, key: Key)
+  {
+    && r.Const?
+    && r.v.key == key
+  }
+
+  function CountConsts(m: multiset<R>, key: Key) : nat
+  {
+    MultisetUtil.Count((r) => is_const(r, key), m)
+  }
+
+  predicate InvGlobal(g: map<Key, RWLockState>, m: multiset<R>)
+  {
+    && (forall key | key in g :: InvRWLockState(key, g[key], m))
   }
 
   predicate InvObjectState(key: Key, q: Q, state: RWLockState)
   {
-    && InvRWLockState(key, state)
+    && |state.readCounts| == NUM_THREADS
     && (q.FlagsField? ==>
       && (q.flags == Unmapped ==>
         && state.unmapped
@@ -383,11 +384,11 @@ module RWLock refines ResourceBuilderSpec {
         && !state.excState.clean
       )
       && (q.flags == WriteBack_PendingExcLock ==>
-        && state.excState == WLSPendingAwaitWriteBack
+        && state.excState.WLSPendingAwaitWriteBack?
         && state.backHeld
       )
       && (q.flags == PendingExcLock ==>
-        && state.excState == WLSPendingAwaitWriteBack
+        && state.excState.WLSPendingAwaitWriteBack?
         && !state.backHeld
       )
     )
@@ -406,7 +407,7 @@ module RWLock refines ResourceBuilderSpec {
     )
 
     && (q.ExcLockPendingAwaitWriteBack? ==>
-      && state.excState == WLSPendingAwaitWriteBack
+      && state.excState == WLSPendingAwaitWriteBack(q.t)
     )
     && (q.ExcLockPending? ==>
       && state.excState == WLSPending(q.t, q.visited, q.clean)
@@ -430,18 +431,23 @@ module RWLock refines ResourceBuilderSpec {
     )
   }
 
-  predicate InvObject(q: R, g: map<Key, RWLockState>)
+  predicate InvObject(r: R, g: map<Key, RWLockState>)
   {
-    && q.Internal?
-    && !q.q.Global?
-    && q.q.key in g
-    && InvObjectState(q.q.key, q.q, g[q.q.key])
+    && (r.Internal? ==> (
+      && !r.q.Global?
+      && r.q.key in g
+      && InvObjectState(r.q.key, r.q, g[r.q.key])
+    ))
+    && (r.Const? ==> (
+      && r.v.key in g
+      && g[r.v.key].handle == Some(r.v)
+    ))
   }
 
   predicate Inv2(q: R, r: R)
   {
-    && q.Internal? ==> (
-      && r.Internal? ==> (
+    && (q.Internal? ==> (
+      && (r.Internal? ==> (
         && !(q.q.Global? && r.q.Global?)
         && (q.q.FlagsField? && r.q.FlagsField? ==> q.q.key != r.q.key)
         && (q.q.SharedLockRefCount? && r.q.SharedLockRefCount? ==> !(q.q.key == r.q.key && q.q.t == r.q.t))
@@ -449,18 +455,31 @@ module RWLock refines ResourceBuilderSpec {
         && (q.q.ExcLockPendingAwaitWriteBack? && r.q.ExcLockPendingAwaitWriteBack? ==> q.q.key != r.q.key)
         && (q.q.ExcLockPending? && r.q.ExcLockPending? ==> q.q.key != r.q.key)
         && (q.q.ExcLockObtained? && r.q.ExcLockObtained? ==> q.q.key != r.q.key)
-        && (q.q.Global? ==>
-          && InvObject(r, q.q.g)
-        )
-      )
-    )
+      ))
+      && (q.q.Global? ==> (
+        && InvObject(r, q.q.g)
+      ))
+    ))
   }
 
   predicate Inv(s: Variables)
   {
-    && (forall g | g in s.m :: g.Internal? && g.q.Global? ==> InvGlobal(g.q.g))
+    && (forall g | g in s.m :: g.Internal? && g.q.Global? ==> InvGlobal(g.q.g, s.m))
     && (forall a, b | multiset{a,b} <= s.m :: Inv2(a, b))
+    && (forall key :: CountConsts(s.m, key) == CountConstRefs(s.m, key))
   }
+
+  lemma forall_CountReduce<A>()
+  ensures forall fn: A->bool, a, b {:trigger Count<A>(fn, a + b) }
+    :: Count<A>(fn, a + b) == Count<A>(fn, a) + Count<A>(fn, b)
+  ensures forall fn: A->bool, a {:trigger Count<A>(fn, multiset{a}) }
+    :: Count<A>(fn, multiset{a}) == (if fn(a) then 1 else 0)
+  ensures forall fn: A->bool, a, b {:trigger Count<A>(fn, multiset{a,b}) }
+    :: Count<A>(fn, multiset{a,b}) ==
+        (if fn(a) then 1 else 0) + (if fn(b) then 1 else 0)
+  ensures forall fn: A->bool, a, b, c {:trigger Count<A>(fn, multiset{a,b, c}) }
+    :: Count<A>(fn, multiset{a,b,c}) ==
+        (if fn(a) then 1 else 0) + (if fn(b) then 1 else 0) + (if fn(c) then 1 else 0)
 
   // Relevant assertions to trigger all relevant Inv2(x, y) expressions
   lemma UsefulTriggers(
@@ -493,9 +512,12 @@ module RWLock refines ResourceBuilderSpec {
   ensures Inv(s')
   {
     UsefulTriggers(s, s', step, a, a', rest);
+    forall_CountReduce<R>();
 
-    assert InvRWLockState(step.key, step.state);
-    assert InvRWLockState(step.key, step.state');
+    assert InvRWLockState(step.key, step.state, s.m);
+    assert InvRWLockState(step.key, step.state', s'.m);
+
+    //assert step.state.handle.Some?;
 
     forall q, p | multiset{q, p} <= s'.m
     ensures Inv2(q, p)
@@ -509,6 +531,12 @@ module RWLock refines ResourceBuilderSpec {
       } else if multiset{q, p} <= a' {
         assert Inv2(q, p);
       }
+    }
+
+    forall k
+    ensures CountConsts(s'.m, k) == CountConstRefs(s'.m, k)
+    {
+      assert CountConsts(s.m, k) == CountConstRefs(s.m, k); // trigger
     }
   }
 
@@ -524,9 +552,15 @@ module RWLock refines ResourceBuilderSpec {
   ensures Inv(s')
   {
     UsefulTriggers(s, s', step, a, a', rest);
+    forall_CountReduce<R>();
 
-    assert InvRWLockState(step.key, step.state);
-    assert InvRWLockState(step.key, step.state');
+    assert InvRWLockState(step.key, step.state, s.m);
+    assert InvRWLockState(step.key, step.state', s'.m);
+
+    forall g | g in s'.m && g.Internal? && g.q.Global?
+    ensures InvGlobal(g.q.g, s'.m)
+    {
+    }
 
     forall q, p | multiset{q, p} <= s'.m
     ensures Inv2(q, p)
@@ -540,6 +574,137 @@ module RWLock refines ResourceBuilderSpec {
       } else if multiset{q, p} <= a' {
         assert Inv2(q, p);
       }
+    }
+
+    forall k
+    ensures CountConsts(s'.m, k) == CountConstRefs(s'.m, k)
+    {
+      assert CountConsts(s.m, k) == CountConstRefs(s.m, k); // trigger
+    }
+  }
+
+  lemma TakeExcLockFinishWriteBackStepPreservesInv(
+      s: Variables, s': Variables, step: QStep,
+      a: multiset<R>, a': multiset<R>, rest: multiset<R>)
+  requires s'.saved == s.saved
+  requires s.m == a + rest
+  requires s'.m == a' + rest
+  requires transform_step(a, a', step)
+  requires Inv(s)
+  requires step.basicStep.TakeExcLockFinishWriteBackStep?
+  ensures Inv(s')
+  {
+    UsefulTriggers(s, s', step, a, a', rest);
+    forall_CountReduce<R>();
+
+    assert InvRWLockState(step.key, step.state, s.m);
+    assert InvRWLockState(step.key, step.state', s'.m);
+
+    forall q, p | multiset{q, p} <= s'.m
+    ensures Inv2(q, p)
+    {
+      if multiset{q, p} <= rest {
+        assert Inv2(q, p);
+      } else if q in a' && p in rest {
+        assert Inv2(q, p);
+      } else if q in rest && p in a' {
+        assert Inv2(q, p);
+      } else if multiset{q, p} <= a' {
+        assert Inv2(q, p);
+      }
+    }
+
+    forall k
+    ensures CountConsts(s'.m, k) == CountConstRefs(s'.m, k)
+    {
+      assert CountConsts(s.m, k) == CountConstRefs(s.m, k); // trigger
+    }
+  }
+
+  lemma TakeExcLockSharedLockZeroStepPreservesInv(
+      s: Variables, s': Variables, step: QStep,
+      a: multiset<R>, a': multiset<R>, rest: multiset<R>)
+  requires s'.saved == s.saved
+  requires s.m == a + rest
+  requires s'.m == a' + rest
+  requires transform_step(a, a', step)
+  requires Inv(s)
+  requires step.basicStep.TakeExcLockSharedLockZeroStep?
+  ensures Inv(s')
+  {
+    UsefulTriggers(s, s', step, a, a', rest);
+    forall_CountReduce<R>();
+
+    assert InvRWLockState(step.key, step.state, s.m);
+    assert InvRWLockState(step.key, step.state', s'.m);
+
+    forall q, p | multiset{q, p} <= s'.m
+    ensures Inv2(q, p)
+    {
+      if multiset{q, p} <= rest {
+        assert Inv2(q, p);
+      } else if q in a' && p in rest {
+        assert Inv2(q, p);
+      } else if q in rest && p in a' {
+        assert Inv2(q, p);
+      } else if multiset{q, p} <= a' {
+        assert Inv2(q, p);
+      }
+    }
+
+    forall k
+    ensures CountConsts(s'.m, k) == CountConstRefs(s'.m, k)
+    {
+      assert CountConsts(s.m, k) == CountConstRefs(s.m, k); // trigger
+    }
+  }
+
+  lemma TakeExcLockFinishStepPreservesInv(
+      s: Variables, s': Variables, step: QStep,
+      a: multiset<R>, a': multiset<R>, rest: multiset<R>)
+  requires s'.saved == s.saved
+  requires s.m == a + rest
+  requires s'.m == a' + rest
+  requires transform_step(a, a', step)
+  requires Inv(s)
+  requires step.basicStep.TakeExcLockFinishStep?
+  ensures Inv(s')
+  {
+    UsefulTriggers(s, s', step, a, a', rest);
+    forall_CountReduce<R>();
+
+    assert InvRWLockState(step.key, step.state, s.m);
+    assert InvRWLockState(step.key, step.state', s'.m);
+
+    forall q, p | multiset{q, p} <= s'.m
+    ensures Inv2(q, p)
+    {
+      if multiset{q, p} <= rest {
+        assert Inv2(q, p);
+      } else if q in a' && p in rest {
+        if p.Const? && p.v.key == step.key {
+          // If a Const exists, then there is either
+          // a SharedObtained or a WriteBackObtained object
+          // to certify it, and that would lead to a contradiction.
+          Count_ge_1((r) => is_const(r, step.key), s.m, p);
+          assert CountConsts(s.m, step.key)
+              == CountConstRefs(s.m, step.key);
+          var o := get_true_elem((r) => is_const_ref(r, step.key), s.m);
+          assert false;
+        }
+
+        assert Inv2(q, p);
+      } else if q in rest && p in a' {
+        assert Inv2(q, p);
+      } else if multiset{q, p} <= a' {
+        assert Inv2(q, p);
+      }
+    }
+
+    forall k
+    ensures CountConsts(s'.m, k) == CountConstRefs(s'.m, k)
+    {
+      assert CountConsts(s.m, k) == CountConstRefs(s.m, k); // trigger
     }
   }
 
@@ -559,6 +724,17 @@ module RWLock refines ResourceBuilderSpec {
       }
       case ReleaseWriteBackStep(_,_,_,_,_) => {
         ReleaseWriteBackStepPreservesInv(s, s', step, a, a', rest);
+      }
+      case TakeExcLockFinishWriteBackStep(_,_,_,_,_,_,_) => {
+         TakeExcLockFinishWriteBackStepPreservesInv(
+            s, s', step, a, a', rest);
+      }
+      case TakeExcLockSharedLockZeroStep(_,_,_,_,_,_) => {
+         TakeExcLockSharedLockZeroStepPreservesInv(
+            s, s', step, a, a', rest);
+      }
+      case TakeExcLockFinishStep(_,_,_,_,_) => {
+         TakeExcLockFinishStepPreservesInv(s, s', step, a, a', rest);
       }
     }
   }
